Automation!

Relation.lean
@@ -1,5 +1,75 @@
 open tactic
 
+meta def map: (expr → tactic unit) → list expr → tactic unit
+  | f [] := failed
+  | f (x :: xs) := f x <|> map f xs
+
+meta def size : expr → nat
+| (expr.app f a) := size f + size a
+| _ := 1
+
+meta def sort_of_identifier: expr → string
+ | (expr.var nat) := "var"
+ | (expr.sort level) := "sort"
+ | (expr.const name list_level) := "const"
+ | (expr.mvar unique pretty type) := "mvar"
+ | (expr.local_const unique pretty info type) := "local_const"
+ | (expr.app expr₁ expr₂) := ("apply (" ++ (sort_of_identifier expr₁ ++ " (" ++ to_string expr₁ ++ ")) to " ++ sort_of_identifier expr₂))
+ | (expr.lam name info type body) := "lam"
+ | (expr.pi var_name info var_type body) := "pi"
+ | (expr.elet var_name type assignment body) := "elet"
+ | (expr.macro macro_def list_expr) := "macro"
+
+meta def sort_of_goal: tactic unit := target >>= λ expression, trace (sort_of_identifier expression)
+
+meta def normalize_once: tactic unit :=
+do
+  context ← local_context,
+  map (λ hypothesis, do cases hypothesis, return ()) context
+
+meta def normalize := repeat normalize_once
+
+meta def split_once: tactic unit :=
+do intros, split, return ()
+
+meta def split_all := repeat split_once
+
+meta def triviality := repeat (assumption <|> reflexivity)
+
+meta def existence := do
+  context ← local_context,
+  map (λ hypothesis, do existsi hypothesis) context
+
+meta def is_exists: expr → tactic bool := λ target, do
+  match target with
+    | expr.app (expr.const `Exists _) _ := return tt
+    | expr.app recurse _ := is_exists recurse
+    | _ := return ff
+    end
+
+meta def is_target_exists: tactic bool := do
+  target ← target,
+  is_exists target
+
+meta def slice_and_dice := do
+  target ← target,
+  is_exists_target ← is_exists target,
+  match is_exists_target with
+    | tt := existence
+    | ff := split >> intros >> return ()
+  end
+
+meta def crush_once: tactic unit := do
+  intros, normalize, try (interactive.simp none none tt [ ] [ ] (interactive.loc.ns [none])), repeat (do slice_and_dice >> intros >> return ()), triviality
+
+meta def repeat_safely (operate: tactic unit): tactic unit := do
+  current_target ← target,
+  operate,
+  next_target ← target,
+  (unify current_target next_target >> return ()) <|> operate
+
+meta def crush := repeat crush_once
+
 def ℙ := Prop
 class Same (φ: Type) := (same: φ → φ → ℙ)
 notation x `≡` y := Same.same x y
@@ -15,47 +85,33 @@ local notation r₂ `∘` r₁ := compose r₁ r₂
 
 theorem has_left_identity (α β: Type): ∀ (r: α ~ β), identity ∘ r ≡ r :=
 begin
-  intros,unfold identity, unfold compose,
+  intros, unfold identity, unfold compose,
   dsimp {md := transparency.instances},
-  intros x y, split,
-      intro H, cases H with x' proof, cases proof, subst proof_right, apply proof_left,
-      intro H, existsi y, split,
-        assumption,
-        reflexivity,
+  crush,
 end
 
 theorem has_right_identity (α β: Type): ∀ (r: α ~ β), r ∘ identity ≡ r :=
 begin
-  intros,unfold identity, unfold compose,
+  intros, unfold identity, unfold compose,
   dsimp {md := transparency.instances},
-  intros, split,
-    intro H, cases H with x' proof, cases proof, subst proof_left, apply proof_right,
-    intro H, existsi x, split,
-      reflexivity,
-      assumption,
+  crush,
 end
 
-meta def map: (expr → tactic unit) → list expr → tactic unit
-  | f [] := failed
-  | f (x :: xs) := f x <|> map f xs
+theorem has_identity (α β: Type): ∀ (r: α ~ β), (identity ∘ r ≡ r) ∧ (r ∘ identity ≡ r) :=
+begin
+  intros, unfold identity, unfold compose,
+  dsimp {md := transparency.instances},
+  crush,
+end
 
-meta def normalize_once: tactic unit :=
-do
-  context ← local_context,
-  map (λ hypothesis, do cases hypothesis, return ()) context
+#check interactive.existsi
 
-meta def normalize := repeat normalize_once
-
-meta def split_once: tactic unit :=
-do intros, split, return ()
-
-meta def split_all := repeat split_once
-
-meta def triviality := repeat assumption
-
-meta def existence := do
-  context ← local_context,
-  map (λ hypothesis, do existsi hypothesis) context
+theorem exists_identity (α β: Type): ∀ (r: α ~ β), ∃ (ε: ∀ (type: Type), type ~ type), (ε β ∘ r ≡ r) ∧ (r ∘ ε α ≡ r) :=
+begin
+  intros, unfold compose,
+  dsimp {md := transparency.instances},
+  existsi (λ τ x y, x = y), crush,
+end
 
 theorem compose_is_associative (α β γ δ: Type)
   : ∀ (r₁: α ~ β) (r₂: β ~ γ) (r₃: γ ~ δ)
@@ -63,7 +119,5 @@ theorem compose_is_associative (α β γ δ: Type)
 begin
   intros, unfold compose,
   dsimp {md := transparency.instances},
-  intros x₁ x₄, split,
-    { intros, normalize, existence, split, existence, split, triviality },
-    { intros, normalize, existence, split, assumption, existence, split, triviality },
+  crush,
 end
